Flesh out the code some more.

Janus.v
@@ -3,11 +3,13 @@
 (* Current implementation is highly partial *)
 Require Import Arith.
 Require Import ZArith.
+Require Import Bool.
 Require Import MemMonad.
 
 
 Section Janus.
   Open Scope Z_scope.
+
   Inductive Exp : Set :=
   | E_Const : Z -> Exp
   | E_Var   : nat -> Exp
@@ -23,4 +25,80 @@ Section Janus.
       | E_Minus e1 e2 => denoteExp m e1 - denoteExp m e2
       | E_Mul e1 e2 => denoteExp m e1 * denoteExp m e2
     end.
+
+  Inductive BExp : Set :=
+  | B_Eq  : Exp -> Exp -> BExp
+  | B_Neq : Exp -> Exp -> BExp
+  | B_LT  : Exp -> Exp -> BExp
+  | B_And : BExp -> BExp -> BExp
+  | B_Or  : BExp -> BExp -> BExp.
+
+  Fixpoint denoteBExp (m : memory) (e : BExp) {struct e} : bool :=
+    match e with
+      | B_Eq e1 e2 =>
+        if Z_eq_dec (denoteExp m e1) (denoteExp m e2)
+          then true
+          else false
+      | B_Neq e1 e2 =>
+        if Z_eq_dec (denoteExp m e1) (denoteExp m e2)
+          then false
+          else true
+      | B_LT e1 e2 =>
+        match Zcompare (denoteExp m e1) (denoteExp m e2) with
+        |  Lt => true
+        |  _  => false
+        end
+      | B_And b1 b2 => andb (denoteBExp m b1) (denoteBExp m b2)
+      | B_Or b1 b2  => orb (denoteBExp m b1) (denoteBExp m b2)
+    end.
+
+  Inductive Stmt : Set :=
+  | S_Incr : var -> Exp -> Stmt
+  | S_Decr : var -> Exp -> Stmt
+  | S_Swap : var -> var -> Stmt
+  | S_If : BExp -> Stmt -> Stmt -> BExp -> Stmt
+  | S_Semi : Stmt -> Stmt -> Stmt.
+
+
+  Fixpoint denoteStmt (s : Stmt) : memM unit :=
+    match s with
+      | S_Incr v e =>
+        (fun m =>
+          (r <- Return (denoteExp m e);
+            r' <- Read v ;
+            Write v (r + r')) m)
+      | S_Decr v e =>
+        (fun m =>
+          (r <- Return (denoteExp m e);
+            r' <- Read v ;
+            Write v (r - r')) m)
+      | S_Swap v1 v2 =>
+        r1 <- Read v1 ;
+        r2 <- Read v2 ;
+        Write v1 r2 ;;
+        Write v2 r1
+      | S_Semi s1 s2 => (denoteStmt s1) ;; (denoteStmt s2)
+      | S_If b t e a =>
+        (fun m =>
+          (* Wrong at the moment *)
+          (if (denoteBExp m b)
+            then denoteStmt t
+            else denoteStmt e) m)
+    end.
+
+    Fixpoint invert (s : Stmt) : Stmt :=
+      match s with
+        | S_Incr v e => S_Decr v e
+        | S_Decr v e => S_Incr v e
+        | S_Swap v1 v2 => S_Swap v1 v2
+        | S_If b t f a => S_If a (invert t) (invert f) b
+        | S_Semi s1 s2 => S_Semi (invert s2) (invert s1)
+      end.
+
+    Theorem invert_self_inverse :
+      forall s, invert (invert s) = s.
+      induction s; intuition;
+      simpl; rewrite IHs1; rewrite IHs2; reflexivity.
+    Qed.
+
 End Janus.
